keccak: more progress on the verification

Garden/Plonky3/keccak/air_local.v
@@ -5,88 +5,88 @@ Require Import Garden.Plonky3.keccak.constants.
 
 (** In this definition, we group all the constraints about the current [local] row. *)
 Definition eval_local {p} `{Prime p} (local : KeccakCols.t) : M.t unit :=
-  let* _ := eval_preimage_a local in
-  let* _ := eval_assert_export_bool local in
-  let* _ := eval_assert_export_zero local in
-  let* _ := eval_assert_c_c_prime local in
-  let* _ := eval_assert_a_a_prime_c_c_prime local in
-  let* _ := eval_assert_a_prime_c_prime local in
-  let* _ := eval_assert_a_prime_prime local in
-  let* _ := eval_assert_a_prime_prime_0_0_bits_bools local in
-  let* _ := eval_assert_a_prime_prime_0_0_limbs local in
-  let* _ := eval_assert_a_prime_prime_prime_0_0_limbs local in
+  let* _ := preimage_a.eval local in
+  let* _ := export_bool.eval local in
+  let* _ := export_zero.eval local in
+  let* _ := c_c_prime.eval local in
+  let* _ := a_a_prime_c_c_prime.eval local in
+  let* _ := a_prime_c_prime.eval local in
+  let* _ := a_prime_prime.eval local in
+  let* _ := a_prime_prime_0_0_bits_bools.eval local in
+  let* _ := a_prime_prime_0_0_limbs.eval local in
+  let* _ := a_prime_prime_prime_0_0_limbs.eval local in
   M.pure tt.
-
-Module KeccakCols.
-  Definition get_a (local : KeccakCols.t) (y x z : Z) : bool :=
-    Limbs.get_bit BITS_PER_LIMB ((local.(KeccakCols.a).(Array.get) y).(Array.get) x) z.
-
-  Definition get_c (local : KeccakCols.t) (x z : Z) : bool :=
-    Z.odd ((local.(KeccakCols.c).(Array.get) x).(Array.get) z).
-
-  Definition get_c_prime (local : KeccakCols.t) (x z : Z) : bool :=
-    Z.odd ((local.(KeccakCols.c_prime).(Array.get) x).(Array.get) z).
-
-  Definition get_a_prime (local : KeccakCols.t) (y x z : Z) : bool :=
-    Z.odd (((local.(KeccakCols.a_prime).(Array.get) y).(Array.get) x).(Array.get) z).
-End KeccakCols.
 
 Definition xorbs (bs : list bool) : bool :=
   Lists.List.fold_left xorb bs false.
 
 Module FirstRowsFrom_a.
   Module From.
-    Record t (local : KeccakCols.t) : Set := {
+    Record t (local : KeccakCols.t) : Prop := {
       c_c_prime (x z : Z) :
-        KeccakCols.get_c_prime local x z =
+        0 <= x < 5 ->
+        0 <= z < 64 ->
+        KeccakCols.Bool.get_c_prime local x z =
         xorbs [
-          KeccakCols.get_c local x z;
-          KeccakCols.get_c local ((x + 4) mod 5) z;
-          KeccakCols.get_c local ((x + 1) mod 5) ((z + 63) mod 64)
+          KeccakCols.Bool.get_c local x z;
+          KeccakCols.Bool.get_c local ((x + 4) mod 5) z;
+          KeccakCols.Bool.get_c local ((x + 1) mod 5) ((z + 63) mod 64)
         ];
       a_a_prime_c_c_prime (x y z : Z) :
-        KeccakCols.get_a local x y z =
+        0 <= x < 5 ->
+        0 <= y < 5 ->
+        0 <= z < 64 ->
+        KeccakCols.Bool.get_a local x y z =
         xorbs [
-          KeccakCols.get_a_prime local x y z;
-          KeccakCols.get_c local x z;
-          KeccakCols.get_c_prime local x z
+          KeccakCols.Bool.get_a_prime local x y z;
+          KeccakCols.Bool.get_c local x z;
+          KeccakCols.Bool.get_c_prime local x z
         ];
       a_prime_c_prime (x z : Z) :
-        KeccakCols.get_c_prime local x z =
+        0 <= x < 5 ->
+        0 <= z < 64 ->
+        KeccakCols.Bool.get_c_prime local x z =
         xorbs [
-          KeccakCols.get_a_prime local x 0 z;
-          KeccakCols.get_a_prime local x 1 z;
-          KeccakCols.get_a_prime local x 2 z;
-          KeccakCols.get_a_prime local x 3 z;
-          KeccakCols.get_a_prime local x 4 z
+          KeccakCols.Bool.get_a_prime local x 0 z;
+          KeccakCols.Bool.get_a_prime local x 1 z;
+          KeccakCols.Bool.get_a_prime local x 2 z;
+          KeccakCols.Bool.get_a_prime local x 3 z;
+          KeccakCols.Bool.get_a_prime local x 4 z
         ];
     }.
   End From.
 
   Module To.
-    Record t (local : KeccakCols.t) : Set := {
+    Record t (local : KeccakCols.t) : Prop := {
       a_c (x z : Z) :
-        KeccakCols.get_c local x z =
+        0 <= x < 5 ->
+        0 <= z < 64 ->
+        KeccakCols.Bool.get_c local x z =
         xorbs [
-          KeccakCols.get_a local x 0 z;
-          KeccakCols.get_a local x 1 z;
-          KeccakCols.get_a local x 2 z;
-          KeccakCols.get_a local x 3 z;
-          KeccakCols.get_a local x 4 z
+          KeccakCols.Bool.get_a local x 0 z;
+          KeccakCols.Bool.get_a local x 1 z;
+          KeccakCols.Bool.get_a local x 2 z;
+          KeccakCols.Bool.get_a local x 3 z;
+          KeccakCols.Bool.get_a local x 4 z
         ];
       c_c_prime (x z : Z) :
-        KeccakCols.get_c_prime local x z =
+        0 <= x < 5 ->
+        0 <= z < 64 ->
+        KeccakCols.Bool.get_c_prime local x z =
         xorbs [
-          KeccakCols.get_c local x z;
-          KeccakCols.get_c local ((x + 4) mod 5) z;
-          KeccakCols.get_c local ((x + 1) mod 5) ((z + 63) mod 64)
+          KeccakCols.Bool.get_c local x z;
+          KeccakCols.Bool.get_c local ((x + 4) mod 5) z;
+          KeccakCols.Bool.get_c local ((x + 1) mod 5) ((z + 63) mod 64)
         ];
       a_a_prime_c (x y z : Z) :
-        KeccakCols.get_a_prime local x y z =
+        0 <= x < 5 ->
+        0 <= y < 5 ->
+        0 <= z < 64 ->
+        KeccakCols.Bool.get_a_prime local x y z =
         xorbs [
-          KeccakCols.get_a local x y z;
-          KeccakCols.get_c local ((x + 4) mod 5) z;
-          KeccakCols.get_c local ((x + 1) mod 5) ((z + 63) mod 64)
+          KeccakCols.Bool.get_a local x y z;
+          KeccakCols.Bool.get_c local ((x + 4) mod 5) z;
+          KeccakCols.Bool.get_c local ((x + 1) mod 5) ((z + 63) mod 64)
         ];
     }.
   End To.
@@ -97,17 +97,17 @@ Module FirstRowsFrom_a.
     To.t local.
   Proof.
     intros []; constructor; intros; cbn in *.
-    { repeat rewrite a_a_prime_c_c_prime.
-      repeat rewrite a_prime_c_prime.
-      repeat destruct (KeccakCols.get_c _);
-        repeat destruct (KeccakCols.get_a_prime _);
+    { repeat rewrite a_a_prime_c_c_prime by lia.
+      repeat rewrite a_prime_c_prime by lia.
+      repeat destruct (KeccakCols.Bool.get_c _);
+        repeat destruct (KeccakCols.Bool.get_a_prime _);
         reflexivity.
     }
-    { congruence. }
-    { rewrite a_a_prime_c_c_prime.
-      rewrite c_c_prime.
-      repeat destruct (KeccakCols.get_a_prime _);
-        repeat destruct (KeccakCols.get_c _);
+    { hauto l: on. }
+    { rewrite a_a_prime_c_c_prime by lia.
+      rewrite c_c_prime by lia.
+      repeat destruct (KeccakCols.Bool.get_a_prime _);
+        repeat destruct (KeccakCols.Bool.get_c _);
         reflexivity.
     }
   Qed.
@@ -118,26 +118,113 @@ Lemma xor_sum_diff_eq (local : KeccakCols.t) (x z : Z)
   (H_sum_diff :
     let diff :=
       Lists.List.fold_left Z.add [
-        Z.b2z (KeccakCols.get_a_prime local x 0 z);
-        Z.b2z (KeccakCols.get_a_prime local x 1 z);
-        Z.b2z (KeccakCols.get_a_prime local x 2 z);
-        Z.b2z (KeccakCols.get_a_prime local x 3 z);
-        Z.b2z (KeccakCols.get_a_prime local x 4 z)
+        Z.b2z (KeccakCols.Bool.get_a_prime local x 0 z);
+        Z.b2z (KeccakCols.Bool.get_a_prime local x 1 z);
+        Z.b2z (KeccakCols.Bool.get_a_prime local x 2 z);
+        Z.b2z (KeccakCols.Bool.get_a_prime local x 3 z);
+        Z.b2z (KeccakCols.Bool.get_a_prime local x 4 z)
       ] 0 -
-      Z.b2z (KeccakCols.get_c_prime local x z) in
+      Z.b2z (KeccakCols.Bool.get_c_prime local x z) in
     diff = 0 \/ diff = 2 \/ diff = 4
   ) :
-  KeccakCols.get_c_prime local x z =
+  KeccakCols.Bool.get_c_prime local x z =
   xorbs [
-    KeccakCols.get_a_prime local x 0 z;
-    KeccakCols.get_a_prime local x 1 z;
-    KeccakCols.get_a_prime local x 2 z;
-    KeccakCols.get_a_prime local x 3 z;
-    KeccakCols.get_a_prime local x 4 z
+    KeccakCols.Bool.get_a_prime local x 0 z;
+    KeccakCols.Bool.get_a_prime local x 1 z;
+    KeccakCols.Bool.get_a_prime local x 2 z;
+    KeccakCols.Bool.get_a_prime local x 3 z;
+    KeccakCols.Bool.get_a_prime local x 4 z
   ].
 Proof.
-  destruct (KeccakCols.get_c_prime _);
-    repeat destruct (KeccakCols.get_a_prime _);
+  destruct (KeccakCols.Bool.get_c_prime _);
+    repeat destruct (KeccakCols.Bool.get_a_prime _);
     cbn in *;
     lia.
 Qed.
+
+Lemma odd_b2z_eq (b : bool) :
+  Z.odd (Z.b2z b) = b.
+Proof.
+  destruct b; cbn; reflexivity.
+Qed.
+
+Lemma eval_local_implies {p} `{Prime p} (local : KeccakCols.t) :
+  let local := M.map_mod local in
+  {{ eval_local local 🔽
+    tt,
+    FirstRowsFrom_a.From.t local
+  }}.
+Proof.
+  intros *.
+  unfold eval_local.
+  eapply Run.LetAccumulate with (P1 := True). {
+    admit.
+  }
+  intros [].
+  eapply Run.LetAccumulate with (P1 := True). {
+    admit.
+  }
+  intros [].
+  eapply Run.LetAccumulate with (P1 := True). {
+    admit.
+  }
+  intros [].
+  eapply Run.LetAccumulate. {
+    apply c_c_prime.implies.
+  }
+  intros [].
+  eapply Run.LetAccumulate. {
+    apply a_a_prime_c_c_prime.implies.
+  }
+  intros [].
+  eapply Run.LetAccumulate. {
+    apply a_prime_c_prime.implies.
+  }
+  intros H_eval_assert_a_prime_c_prime.
+  eapply Run.LetAccumulate. {
+    apply a_prime_prime.implies.
+  }
+  intros H_eval_assert_a_prime_prime.
+  eapply Run.LetAccumulate. {
+    apply a_prime_prime_0_0_bits_bools.implies.
+  }
+  intros H_eval_assert_a_prime_prime_0_0_bits_bools.
+  eapply Run.LetAccumulate. {
+    apply a_prime_prime_0_0_limbs.implies.
+  }
+  intros H_eval_assert_a_prime_prime_0_0_limbs.
+  eapply Run.LetAccumulate. {
+    apply a_prime_prime_prime_0_0_limbs.implies.
+  }
+  intros H_eval_assert_a_prime_prime_prime_0_0_limbs.
+  eapply Run.Implies. {
+    apply Run.Pure.
+  }
+  intros [].
+  constructor; intros.
+  { unfold KeccakCols.Bool.get_c, KeccakCols.Bool.get_c_prime.
+    rewrite c_c_prime_eq by lia.
+    repeat rewrite c_bools by lia.
+    rewrite xor3_eq.
+    repeat (cbn || f_equal || rewrite odd_b2z_eq).
+  }
+  { unfold KeccakCols.Bool.get_a.
+    unfold KeccakCols.get_a in a_a_prime_c_c_prime_eq.
+    erewrite Limbs.get_bit_of_bools_eqs; try (unfold U64_LIMBS, BITS_PER_LIMB; lia).
+    3: {
+      intros.
+      apply a_a_prime_c_c_prime_eq; lia.
+    }
+    2: {
+      intros.
+      unfold a_a_prime_c_c_prime.get_bit.
+      admit.
+    }
+    unfold a_a_prime_c_c_prime.get_bit.
+    cbn.
+    admit.
+  }
+  { apply xor_sum_diff_eq.
+    admit.
+  }
+Admitted.
