Garden/Plonky3/keccak/air_small_parts.v
@@ -13,48 +13,50 @@ Require Import Garden.Plonky3.keccak.constants.
       }
   }
 *)
-Definition eval_preimage_a {p} `{Prime p} (local : KeccakCols.t) : M.t unit :=
-  let first_step := local.(KeccakCols.step_flags).(Array.get) 0 in
-  M.for_in_zero_to_n 5 (fun y =>
-  M.for_in_zero_to_n 5 (fun x =>
-    M.when first_step (
-      M.assert_zeros (N := U64_LIMBS) {|
-        Array.get limb :=
-          BinOp.sub
-            (Array.get (Array.get (Array.get local.(KeccakCols.preimage) y) x) limb)
-            (Array.get (Array.get (Array.get local.(KeccakCols.a) y) x) limb)
-      |}
-    )
-  )).
-
-Lemma eval_preimage_a_implies {p} `{Prime p} (local : KeccakCols.t) :
-    let local := M.map_mod local in
+Module preimage_a.
+  Definition eval {p} `{Prime p} (local : KeccakCols.t) : M.t unit :=
     let first_step := local.(KeccakCols.step_flags).(Array.get) 0 in
-    first_step <> 0 ->
-    {{ eval_preimage_a local 🔽
-      tt,
-      forall (y x limb : Z),
-      0 <= y < 5 ->
-      0 <= x < 5 ->
-      0 <= limb < U64_LIMBS ->
-      ((local.(KeccakCols.preimage).(Array.get) y).(Array.get) x).(Array.get) limb =
-      ((local.(KeccakCols.a).(Array.get) y).(Array.get) x).(Array.get) limb
-    }}.
-Proof.
-  intros * H_not_first_step.
-  eapply Run.Implies. {
-    eapply Run.ForInZeroToN. {
-      intros.
+    M.for_in_zero_to_n 5 (fun y =>
+    M.for_in_zero_to_n 5 (fun x =>
+      M.when first_step (
+        M.assert_zeros (N := U64_LIMBS) {|
+          Array.get limb :=
+            BinOp.sub
+              (Array.get (Array.get (Array.get local.(KeccakCols.preimage) y) x) limb)
+              (Array.get (Array.get (Array.get local.(KeccakCols.a) y) x) limb)
+        |}
+      )
+    )).
+
+  Lemma implies {p} `{Prime p} (local : KeccakCols.t) :
+      let local := M.map_mod local in
+      let first_step := local.(KeccakCols.step_flags).(Array.get) 0 in
+      first_step <> 0 ->
+      {{ eval local 🔽
+        tt,
+        forall (y x limb : Z),
+        0 <= y < 5 ->
+        0 <= x < 5 ->
+        0 <= limb < U64_LIMBS ->
+        KeccakCols.get_preimage local x y limb =
+        KeccakCols.get_a local x y limb
+      }}.
+  Proof.
+    intros * H_not_first_step.
+    eapply Run.Implies. {
       eapply Run.ForInZeroToN. {
         intros.
-        unfold M.when.
-        destruct (_ =? 0) eqn:H_first_step_eq; [lia|].
-        apply Run.AssertZerosFromFnSub.
+        eapply Run.ForInZeroToN. {
+          intros.
+          unfold M.when.
+          destruct (_ =? 0) eqn:H_first_step_eq; [lia|].
+          apply Run.AssertZerosFromFnSub.
+        }
       }
     }
-  }
-  hauto l: on drew: off.
-Qed.
+    hauto l: on drew: off.
+  Qed.
+End preimage_a.
 
 (*
   for y in 0..5 {
@@ -68,115 +70,121 @@ Qed.
       }
   }
 *)
-Definition eval_preimage_next_preimage {p} `{Prime p}
-    (local next : KeccakCols.t)
-    (is_transition : bool) :
-    M.t unit :=
-  let final_step := local.(KeccakCols.step_flags).(Array.get) (NUM_ROUNDS - 1) in
-  let not_final_step := BinOp.sub 1 final_step in
-  M.for_in_zero_to_n 5 (fun y =>
-  M.for_in_zero_to_n 5 (fun x =>
-    M.when not_final_step (
-    M.when_bool is_transition (
-      M.assert_zeros (N := U64_LIMBS) {|
-        Array.get limb :=
-          BinOp.sub
-            (Array.get (Array.get (Array.get local.(KeccakCols.preimage) y) x) limb)
-            (Array.get (Array.get (Array.get next.(KeccakCols.preimage) y) x) limb)
-      |}
-    )
-  ))).
-
-Lemma eval_preimage_next_preimage_transition_implies {p} `{Prime p}
-    (local next : KeccakCols.t) :
-    let local := M.map_mod local in
-    let next := M.map_mod next in
+Module preimage_next_preimage.
+  Definition eval {p} `{Prime p}
+      (local next : KeccakCols.t)
+      (is_transition : bool) :
+      M.t unit :=
     let final_step := local.(KeccakCols.step_flags).(Array.get) (NUM_ROUNDS - 1) in
     let not_final_step := BinOp.sub 1 final_step in
-    not_final_step <> 0 ->
-    {{ eval_preimage_next_preimage local next true 🔽
-      tt,
-      forall (y x limb : Z),
-      0 <= y < 5 ->
-      0 <= x < 5 ->
-      0 <= limb < U64_LIMBS ->
-      ((local.(KeccakCols.preimage).(Array.get) y).(Array.get) x).(Array.get) limb =
-      ((next.(KeccakCols.preimage).(Array.get) y).(Array.get) x).(Array.get) limb
-    }}.
-Proof.
-  intros * H_not_final_step.
-  eapply Run.Implies. {
-    eapply Run.ForInZeroToN. {
-      intros.
+    M.for_in_zero_to_n 5 (fun y =>
+    M.for_in_zero_to_n 5 (fun x =>
+      M.when not_final_step (
+      M.when_bool is_transition (
+        M.assert_zeros (N := U64_LIMBS) {|
+          Array.get limb :=
+            BinOp.sub
+              (Array.get (Array.get (Array.get local.(KeccakCols.preimage) y) x) limb)
+              (Array.get (Array.get (Array.get next.(KeccakCols.preimage) y) x) limb)
+        |}
+      )
+    ))).
+
+  Lemma implies {p} `{Prime p}
+      (local next : KeccakCols.t) :
+      let local := M.map_mod local in
+      let next := M.map_mod next in
+      let final_step := local.(KeccakCols.step_flags).(Array.get) (NUM_ROUNDS - 1) in
+      let not_final_step := BinOp.sub 1 final_step in
+      not_final_step <> 0 ->
+      {{ eval local next true 🔽
+        tt,
+        forall (y x limb : Z),
+        0 <= y < 5 ->
+        0 <= x < 5 ->
+        0 <= limb < U64_LIMBS ->
+        KeccakCols.get_preimage local x y limb =
+        KeccakCols.get_preimage next x y limb
+      }}.
+  Proof.
+    intros * H_not_final_step.
+    eapply Run.Implies. {
       eapply Run.ForInZeroToN. {
         intros.
-        unfold M.when.
-        unfold not_final_step, final_step in *.
-        destruct (_ =? 0) eqn:H_not_final_step_eq; [lia|].
-        apply Run.AssertZerosFromFnSub.
+        eapply Run.ForInZeroToN. {
+          intros.
+          unfold M.when.
+          unfold not_final_step, final_step in *.
+          destruct (_ =? 0) eqn:H_not_final_step_eq; [lia|].
+          apply Run.AssertZerosFromFnSub.
+        }
       }
     }
-  }
-  hauto l: on drew: off.
-Qed.
+    hauto l: on drew: off.
+  Qed.
+End preimage_next_preimage.
 
 (*
   builder.assert_bool(local.export);
 *)
-Definition eval_assert_export_bool {p} `{Prime p}
-    (local : KeccakCols.t) :
-    M.t unit :=
-  M.assert_bool local.(KeccakCols.export). 
+Module export_bool.
+  Definition eval {p} `{Prime p}
+      (local : KeccakCols.t) :
+      M.t unit :=
+    M.assert_bool local.(KeccakCols.export). 
 
-Lemma eval_assert_export_bool_implies {p} `{Prime p}
-    (local : KeccakCols.t) :
-    let local := M.map_mod local in
-  {{
-    eval_assert_export_bool local 🔽
-    tt,
-    exists (b : bool), local.(KeccakCols.export) = Z.b2z b
-  }}.
-Proof.
-  intros.
-  unfold eval_assert_export_bool.
-  apply Run.AssertBool.
-Qed.
+  Lemma implies {p} `{Prime p}
+      (local : KeccakCols.t) :
+      let local := M.map_mod local in
+    {{
+      eval local 🔽
+      tt,
+      local.(KeccakCols.export) =
+      Z.b2z (Z.odd local.(KeccakCols.export))
+    }}.
+  Proof.
+    intros.
+    apply Run.AssertBool.
+  Qed.
+End export_bool.
 
 (*
   builder
     .when(not_final_step.clone())
     .assert_zero(local.export);
 *)
-Definition eval_assert_export_zero {p} `{Prime p}
-    (local : KeccakCols.t) :
-    M.t unit :=
-  let final_step := local.(KeccakCols.step_flags).(Array.get) (NUM_ROUNDS - 1) in
-  let not_final_step := BinOp.sub 1 final_step in
-  M.when not_final_step (
-    M.assert_zero local.(KeccakCols.export)
-  ).
-
-Lemma eval_assert_export_zero_implies {p} `{Prime p}
-    (local : KeccakCols.t) :
-    let local := M.map_mod local in
+Module export_zero.
+  Definition eval {p} `{Prime p}
+      (local : KeccakCols.t) :
+      M.t unit :=
     let final_step := local.(KeccakCols.step_flags).(Array.get) (NUM_ROUNDS - 1) in
     let not_final_step := BinOp.sub 1 final_step in
-    not_final_step <> 0 ->
-    {{ eval_assert_export_zero local 🔽
-      tt,
-      local.(KeccakCols.export) = 0
-    }}.
-Proof.
-  intros.
-  unfold eval_assert_export_zero.
-  eapply Run.Implies. {
-    unfold M.when.
-    unfold not_final_step, final_step in *.
-    destruct (_ =? 0) eqn:H_not_final_step_eq; [lia|].
-    apply Run.Equal.
-  }
-  easy.
-Qed.
+    M.when not_final_step (
+      M.assert_zero local.(KeccakCols.export)
+    ).
+
+  Lemma implies {p} `{Prime p}
+      (local : KeccakCols.t) :
+      let local := M.map_mod local in
+      let final_step := local.(KeccakCols.step_flags).(Array.get) (NUM_ROUNDS - 1) in
+      let not_final_step := BinOp.sub 1 final_step in
+      not_final_step <> 0 ->
+      {{ eval local 🔽
+        tt,
+        local.(KeccakCols.export) = 0
+      }}.
+  Proof.
+    intros.
+    unfold eval.
+    eapply Run.Implies. {
+      unfold M.when.
+      unfold not_final_step, final_step in *.
+      destruct (_ =? 0) eqn:H_not_final_step_eq; [lia|].
+      apply Run.Equal.
+    }
+    easy.
+  Qed.
+End export_zero.
 
 (*
   for x in 0..5 {
@@ -190,67 +198,60 @@ Qed.
       }));
   }
 *)
-Definition eval_assert_c_c_prime {p} `{Prime p}
-    (local : KeccakCols.t) :
-    M.t unit :=
-  M.for_in_zero_to_n 5 (fun x =>
-    let* _ := M.assert_bools (local.(KeccakCols.c).(Array.get) x) in
-    M.assert_zeros (N := 64) {|
-      Array.get z :=
-        let xor :=
-          xor3
-            ((local.(KeccakCols.c).(Array.get) x).(Array.get) z)
-            ((local.(KeccakCols.c).(Array.get) ((x + 4) mod 5)).(Array.get) z)
-            ((local.(KeccakCols.c).(Array.get) ((x + 1) mod 5)).(Array.get) ((z + 63) mod 64))
-        in
-        BinOp.sub
-          ((local.(KeccakCols.c_prime).(Array.get) x).(Array.get) z)
-          xor
-    |}
-  ).
+Module c_c_prime.
+  Definition eval {p} `{Prime p}
+      (local : KeccakCols.t) :
+      M.t unit :=
+    M.for_in_zero_to_n 5 (fun x =>
+      let* _ := M.assert_bools (local.(KeccakCols.c).(Array.get) x) in
+      M.assert_zeros (N := 64) {|
+        Array.get z :=
+          let xor :=
+            xor3
+              ((local.(KeccakCols.c).(Array.get) x).(Array.get) z)
+              ((local.(KeccakCols.c).(Array.get) ((x + 4) mod 5)).(Array.get) z)
+              ((local.(KeccakCols.c).(Array.get) ((x + 1) mod 5)).(Array.get) ((z + 63) mod 64))
+          in
+          BinOp.sub
+            ((local.(KeccakCols.c_prime).(Array.get) x).(Array.get) z)
+            xor
+      |}
+    ).
 
-Lemma eval_assert_c_c_prime_implies_c_bools {p} `{Prime p}
-    (local : KeccakCols.t) :
-    let local := M.map_mod local in
-    {{ eval_assert_c_c_prime local 🔽
-      tt,
-      forall (x z : Z),
-      0 <= x < 5 ->
-      0 <= z < 64 ->
-      exists (b : bool),
-      ((local.(KeccakCols.c).(Array.get) x).(Array.get) z) = Z.b2z b
-    }}.
-Proof.
-  intros.
-  unfold eval_assert_c_c_prime.
-  eapply Run.Implies. {
-    repeat (econstructor || intros).
-  }
-  hauto l: on.
-Qed.
+  Module Valid.
+    Record t {p} `{Prime p} (local : KeccakCols.t) : Prop := {
+      c_c_prime_eq (x z : Z) :
+        0 <= x < 5 ->
+        0 <= z < 64 ->
+        KeccakCols.get_c_prime local x z =
+        M.xor3
+          (KeccakCols.get_c local x z)
+          (KeccakCols.get_c local ((x + 4) mod 5) z)
+          (KeccakCols.get_c local ((x + 1) mod 5) ((z + 63) mod 64));
+      c_bools (x z : Z) :
+        0 <= x < 5 ->
+        0 <= z < 64 ->
+        KeccakCols.get_c local x z =
+        Z.b2z (KeccakCols.Bool.get_c local x z)
+    }.
+  End Valid.
 
-Lemma eval_assert_c_c_prime_implies_c_c_prime {p} `{Prime p}
-    (local : KeccakCols.t) :
-    let local := M.map_mod local in
-    {{ eval_assert_c_c_prime local 🔽
-      tt,
-      forall (x z : Z),
-      0 <= x < 5 ->
-      0 <= z < 64 ->
-      ((local.(KeccakCols.c_prime).(Array.get) x).(Array.get) z) =
-      M.xor3
-        ((local.(KeccakCols.c).(Array.get) x).(Array.get) z)
-        ((local.(KeccakCols.c).(Array.get) ((x + 4) mod 5)).(Array.get) z)
-        ((local.(KeccakCols.c).(Array.get) ((x + 1) mod 5)).(Array.get) ((z + 63) mod 64))
-    }}.
-Proof.
-  intros.
-  unfold eval_assert_c_c_prime.
-  eapply Run.Implies. {
-    repeat (econstructor || intros).
-  }
-  hauto l: on.
-Qed.
+  Lemma implies {p} `{Prime p}
+      (local : KeccakCols.t) :
+      let local := M.map_mod local in
+      {{ eval local 🔽
+        tt,
+        Valid.t local
+      }}.
+  Proof.
+    intros.
+    unfold eval.
+    eapply Run.Implies. {
+      repeat (econstructor || intros).
+    }
+    hauto l: on.
+  Qed.
+End c_c_prime.
 
 (*
   for y in 0..5 {
@@ -277,89 +278,85 @@ Qed.
       }
   }
 *)
-Definition get_big_assert_a_a_prime_c_c_prime {p} `{Prime p}
-    (local : KeccakCols.t) (y x : Z)
-    (z : Z) :
-    Z :=
-  xor3
-    (((local.(KeccakCols.a_prime).(Array.get) y).(Array.get) x).(Array.get) z)
-    ((local.(KeccakCols.c).(Array.get) x).(Array.get) z)
-    ((local.(KeccakCols.c_prime).(Array.get) x).(Array.get) z).
+Module a_a_prime_c_c_prime.
+  Definition get_bit {p} `{Prime p}
+      (local : KeccakCols.t) (y x : Z)
+      (z : Z) :
+      Z :=
+    M.xor3
+      (((local.(KeccakCols.a_prime).(Array.get) y).(Array.get) x).(Array.get) z)
+      ((local.(KeccakCols.c).(Array.get) x).(Array.get) z)
+      ((local.(KeccakCols.c_prime).(Array.get) x).(Array.get) z).
 
-Definition eval_assert_a_a_prime_c_c_prime {p} `{Prime p}
-    (local : KeccakCols.t) :
-    M.t unit :=
-    M.for_in_zero_to_n 5 (fun y =>
-    M.for_in_zero_to_n 5 (fun x =>
-      let* _ := M.assert_bools ((local.(KeccakCols.a_prime).(Array.get) y).(Array.get) x) in
+  Definition eval {p} `{Prime p}
+      (local : KeccakCols.t) :
+      M.t unit :=
+      M.for_in_zero_to_n 5 (fun y =>
+      M.for_in_zero_to_n 5 (fun x =>
+        let* _ := M.assert_bools ((local.(KeccakCols.a_prime).(Array.get) y).(Array.get) x) in
 
-      M.assert_zeros (N := U64_LIMBS) {|
-        Array.get limb :=
-          let computed_limb : Z :=
-            let l : list nat :=
-              List.rev (
-                List.seq
-                  (Z.to_nat (limb * BITS_PER_LIMB))%Z
-                  (Z.to_nat (limb * BITS_PER_LIMB + BITS_PER_LIMB))%Z
-              ) in
-            Lists.List.fold_left (fun acc (z : nat) =>
-              let z : Z := Z.of_nat z in
-              BinOp.add (BinOp.mul 2 acc) (get_big_assert_a_a_prime_c_c_prime local y x z)
-            ) l 0 in
-          BinOp.sub
-            computed_limb
-            (((local.(KeccakCols.a).(Array.get) y).(Array.get) x).(Array.get) limb)
-      |}
-    )).
+        M.assert_zeros (N := U64_LIMBS) {|
+          Array.get limb :=
+            let computed_limb : Z :=
+              let l : list nat :=
+                List.rev (
+                  List.seq
+                    (Z.to_nat (limb * BITS_PER_LIMB))%Z
+                    (Z.to_nat (limb * BITS_PER_LIMB + BITS_PER_LIMB))%Z
+                ) in
+              Lists.List.fold_left (fun acc (z : nat) =>
+                let z : Z := Z.of_nat z in
+                BinOp.add (BinOp.mul 2 acc) (get_bit local y x z)
+              ) l 0 in
+            BinOp.sub
+              computed_limb
+              (((local.(KeccakCols.a).(Array.get) y).(Array.get) x).(Array.get) limb)
+        |}
+      )).
 
-Lemma eval_assert_a_a_prime_c_c_prime_implies_a_prime_bools {p} `{Prime p}
-    (local : KeccakCols.t) :
-    let local := M.map_mod local in
-    {{ eval_assert_a_a_prime_c_c_prime local 🔽
+  Module Valid.
+    Record t {p} `{Prime p} (local : KeccakCols.t) : Prop := {
+      a_prime_bools (x y z : Z) :
+        0 <= x < 5 ->
+        0 <= y < 5 ->
+        0 <= z < 64 ->
+        KeccakCols.get_a_prime local x y z =
+        Z.b2z (KeccakCols.Bool.get_a_prime local x y z);
+      a_a_prime_c_c_prime_eq (x y limb : Z) :
+        0 <= x < 5 ->
+        0 <= y < 5 ->
+        0 <= limb < U64_LIMBS ->
+        let a' : Array.t Z U64_LIMBS :=
+          Limbs.of_bools U64_LIMBS BITS_PER_LIMB {| Array.get z := get_bit local y x z; |} in
+        KeccakCols.get_a local x y limb =
+        a'.(Array.get) limb
+    }.
+  End Valid.
+
+  Lemma implies {p} `{Prime p}
+      (local : KeccakCols.t) :
+      let local := M.map_mod local in
+    {{ eval local 🔽
       tt,
-      forall (y x z : Z),
-      0 <= y < 5 ->
-      0 <= x < 5 ->
-      0 <= z < 64 ->
-      exists (b : bool),
-      ((local.(KeccakCols.a_prime).(Array.get) y).(Array.get) x).(Array.get) z = Z.b2z b
+      Valid.t local
     }}.
-Proof.
-  intros.
-  unfold eval_assert_a_a_prime_c_c_prime.
-  eapply Run.Implies. {
-    repeat (econstructor || intros).
-  }
-  hauto l: on.
-Qed.
-
-Lemma eval_assert_a_a_prime_c_c_prime_implies_a_a_prime_c_c_prime {p} `{Prime p}
-    (local : KeccakCols.t) :
-    let local := M.map_mod local in
-  {{ eval_assert_a_a_prime_c_c_prime local 🔽
-    tt,
-    forall (y x : Z),
-    0 <= y < 5 ->
-    0 <= x < 5 ->
-    let a' : Array.t Z U64_LIMBS :=
-      Limbs.of_bools U64_LIMBS BITS_PER_LIMB
-        {|
-          Array.get z :=
-            get_big_assert_a_a_prime_c_c_prime local y x z;
-        |} in
-    forall (limb : Z),
-    0 <= limb < U64_LIMBS ->
-    ((local.(KeccakCols.a).(Array.get) y).(Array.get) x).(Array.get) limb =
-    a'.(Array.get) limb
-  }}.
-Proof.
-  intros.
-  unfold eval_assert_a_a_prime_c_c_prime.
-  eapply Run.Implies. {
-    repeat (econstructor || intros).
-  }
-  hauto q: on.
-Qed.
+  Proof.
+    intros.
+    unfold eval.
+    eapply Run.Implies. {
+      repeat (econstructor || intros).
+    }
+    unfold Limbs.of_bools; cbn.
+    intros; constructor; intros.
+    { unfold KeccakCols.Bool.get_a_prime; cbn.
+      hauto lq: on rew: off.
+    }
+    { unfold get_bit in *.
+      cbn in *.
+      hauto q: on.
+    }
+  Qed.
+End a_a_prime_c_c_prime.
 
 (*
   for x in 0..5 {
@@ -371,45 +368,54 @@ Qed.
       }));
   }
 *)
-Definition eval_assert_a_prime_c_prime {p} `{Prime p}
-    (local : KeccakCols.t) :
-    M.t unit :=
-  M.for_in_zero_to_n 5 (fun x =>
-    let four : Z := 4 in
-    M.assert_zeros (N := 64) {|
-      Array.get z :=
-        let sum : Z :=
-          Lists.List.fold_left (fun acc y =>
-            BinOp.add acc
-              (Array.get (Array.get (Array.get local.(KeccakCols.a_prime) y) x) z)
-          )
-          (List.map Z.of_nat (List.seq 0 5)) 0 in
-        let diff := BinOp.sub sum (Array.get (Array.get local.(KeccakCols.c_prime) x) z) in
-        BinOp.mul diff (BinOp.mul (BinOp.sub diff 2) (BinOp.sub diff four))
-      |}
-    ).
+Module a_prime_c_prime.
+  Definition eval {p} `{Prime p}
+      (local : KeccakCols.t) :
+      M.t unit :=
+    M.for_in_zero_to_n 5 (fun x =>
+      let four : Z := 4 in
+      M.assert_zeros (N := 64) {|
+        Array.get z :=
+          let sum : Z :=
+            Lists.List.fold_left (fun acc y =>
+              BinOp.add acc
+                (Array.get (Array.get (Array.get local.(KeccakCols.a_prime) y) x) z)
+            )
+            (List.map Z.of_nat (List.seq 0 5)) 0 in
+          let diff := BinOp.sub sum (Array.get (Array.get local.(KeccakCols.c_prime) x) z) in
+          BinOp.mul diff (BinOp.mul (BinOp.sub diff 2) (BinOp.sub diff four))
+        |}
+      ).
 
-Lemma eval_assert_a_prime_c_prime_implies {p} `{Prime p}
-    (local : KeccakCols.t) :
-    let local := M.map_mod local in
-    {{ eval_assert_a_prime_c_prime local 🔽
-      tt,
-      forall (x z : Z),
-      0 <= x < 5 ->
-      0 <= z < 64 ->
-      ((local.(KeccakCols.c_prime).(Array.get) x).(Array.get) z) =
-      M.xor
-        (((local.(KeccakCols.a_prime).(Array.get) x).(Array.get) 0).(Array.get) z)
-        (M.xor
-          (((local.(KeccakCols.a_prime).(Array.get) x).(Array.get) 1).(Array.get) z)
-          (M.xor
-            (((local.(KeccakCols.a_prime).(Array.get) x).(Array.get) 2).(Array.get) z)
-            (((local.(KeccakCols.a_prime).(Array.get) x).(Array.get) 3).(Array.get) z)
-          )
-        )
-    }}.
-Proof.
-Admitted.
+  Lemma implies {p} `{Prime p}
+      (local : KeccakCols.t) :
+      let local := M.map_mod local in
+      {{ eval local 🔽
+        tt,
+        forall (x z : Z),
+        0 <= x < 5 ->
+        0 <= z < 64 ->
+        let diff :=
+          let sum :=
+            Lists.List.fold_left BinOp.add [
+              KeccakCols.get_a_prime local x 0 z;
+              KeccakCols.get_a_prime local x 1 z;
+              KeccakCols.get_a_prime local x 2 z;
+              KeccakCols.get_a_prime local x 3 z;
+              KeccakCols.get_a_prime local x 4 z
+            ] 0 in
+          BinOp.sub sum (KeccakCols.get_c_prime local x z) in
+        BinOp.mul diff (BinOp.mul (BinOp.sub diff 2) (BinOp.sub diff 4)) =
+        0
+      }}.
+  Proof.
+    unfold eval.
+    eapply Run.Implies. {
+      repeat (econstructor || intros).
+    }
+    sauto.
+  Qed.
+End a_prime_c_prime.
 
 (*
   for y in 0..5 {
@@ -430,92 +436,93 @@ Admitted.
       }
   }
 *)
-Definition get_big_assert_a_prime_prime {p} `{Prime p}
-    (local : KeccakCols.t) (y x : Z)
-    (z : Z) :
-    Z :=
-  let andn :=
-    M.andn
-      (Impl_KeccakCols.b local ((x + 1) mod 5) y z)
-      (Impl_KeccakCols.b local ((x + 2) mod 5) y z) in
-  M.xor andn (Impl_KeccakCols.b local x y z).
+Module a_prime_prime.
+  Definition get_bit {p} `{Prime p}
+      (local : KeccakCols.t) (y x : Z)
+      (z : Z) :
+      Z :=
+    let andn :=
+      M.andn
+        (Impl_KeccakCols.b local ((x + 1) mod 5) y z)
+        (Impl_KeccakCols.b local ((x + 2) mod 5) y z) in
+    M.xor andn (Impl_KeccakCols.b local x y z).
 
-Definition eval_assert_a_prime_prime {p} `{Prime p}
-    (local : KeccakCols.t) :
-    M.t unit :=
-  M.for_in_zero_to_n 5 (fun y =>
-  M.for_in_zero_to_n 5 (fun x =>
-    M.assert_zeros (N := U64_LIMBS) {|
-      Array.get limb :=
-        let computed_limb : Z :=
-          let l : list nat :=
-            List.rev (
-              List.seq
-                (Z.to_nat (limb * BITS_PER_LIMB))
-                (Z.to_nat (limb * BITS_PER_LIMB + BITS_PER_LIMB))
-            ) in
-          Lists.List.fold_left (fun acc (z : nat) =>
-            let z : Z := Z.of_nat z in
-            BinOp.add (BinOp.mul 2 acc) (get_big_assert_a_prime_prime local y x z)
-          ) l 0 in
-        BinOp.sub
-          computed_limb
-          (((local.(KeccakCols.a_prime_prime).(Array.get) y).(Array.get) x).(Array.get) limb)
-      |}
-    )).
+  Definition eval {p} `{Prime p}
+      (local : KeccakCols.t) :
+      M.t unit :=
+    M.for_in_zero_to_n 5 (fun y =>
+    M.for_in_zero_to_n 5 (fun x =>
+      M.assert_zeros (N := U64_LIMBS) {|
+        Array.get limb :=
+          let computed_limb : Z :=
+            let l : list nat :=
+              List.rev (
+                List.seq
+                  (Z.to_nat (limb * BITS_PER_LIMB))
+                  (Z.to_nat (limb * BITS_PER_LIMB + BITS_PER_LIMB))
+              ) in
+            Lists.List.fold_left (fun acc (z : nat) =>
+              let z : Z := Z.of_nat z in
+              BinOp.add (BinOp.mul 2 acc) (get_bit local y x z)
+            ) l 0 in
+          BinOp.sub
+            computed_limb
+            (((local.(KeccakCols.a_prime_prime).(Array.get) y).(Array.get) x).(Array.get) limb)
+        |}
+      )).
 
-Lemma eval_assert_a_prime_prime_implies {p} `{Prime p}
-    (local : KeccakCols.t) :
-    let local := M.map_mod local in
-  {{ eval_assert_a_prime_prime local 🔽
-    tt,
-    forall (y x : Z),
-    0 <= y < 5 ->
-    0 <= x < 5 ->
-    let a_prime_prime' : Array.t Z U64_LIMBS :=
-      Limbs.of_bools U64_LIMBS BITS_PER_LIMB
-        {|
-          Array.get z :=
-            get_big_assert_a_prime_prime local y x z;
-        |} in
-    forall (limb : Z),
-    0 <= limb < U64_LIMBS ->
-    ((local.(KeccakCols.a_prime_prime).(Array.get) y).(Array.get) x).(Array.get) limb =
-    a_prime_prime'.(Array.get) limb
-  }}.
-Proof.
-  unfold eval_assert_a_prime_prime.
-  eapply Run.Implies. {
-    repeat (econstructor || intros).
-  }
-  hauto q: on.
-Qed.
+  Lemma implies {p} `{Prime p}
+      (local : KeccakCols.t) :
+      let local := M.map_mod local in
+    {{ eval local 🔽
+      tt,
+      forall (y x : Z),
+      0 <= y < 5 ->
+      0 <= x < 5 ->
+      let a_prime_prime' : Array.t Z U64_LIMBS :=
+        Limbs.of_bools U64_LIMBS BITS_PER_LIMB
+          {| Array.get z := get_bit local y x z; |} in
+      forall (limb : Z),
+      0 <= limb < U64_LIMBS ->
+      KeccakCols.get_a_prime_prime local x y limb =
+      a_prime_prime'.(Array.get) limb
+    }}.
+  Proof.
+    unfold eval.
+    eapply Run.Implies. {
+      repeat (econstructor || intros).
+    }
+    hauto q: on.
+  Qed.
+End a_prime_prime.
 
 (*
   builder.assert_bools(local.a_prime_prime_0_0_bits);
 *)
-Definition eval_assert_a_prime_prime_0_0_bits_bools {p} `{Prime p}
-    (local : KeccakCols.t) :
-    M.t unit :=
-  M.assert_bools local.(KeccakCols.a_prime_prime_0_0_bits).
+Module a_prime_prime_0_0_bits_bools.
+  Definition eval {p} `{Prime p}
+      (local : KeccakCols.t) :
+      M.t unit :=
+    M.assert_bools local.(KeccakCols.a_prime_prime_0_0_bits).
 
-Lemma eval_assert_a_prime_prime_0_0_bits_bools_implies {p} `{Prime p}
-    (local : KeccakCols.t) :
-    let local := M.map_mod local in
-  {{ eval_assert_a_prime_prime_0_0_bits_bools local 🔽
-    tt,
-    forall (z : Z),
-    0 <= z < 64 ->
-    exists (b : bool),
-    (local.(KeccakCols.a_prime_prime_0_0_bits).(Array.get) z) = Z.b2z b
-  }}.
-Proof.
-  unfold eval_assert_a_prime_prime_0_0_bits_bools.
-  eapply Run.Implies. {
-    repeat (econstructor || intros).
-  }
-  sfirstorder.
-Qed.
+  Lemma implies {p} `{Prime p}
+      (local : KeccakCols.t) :
+      let local := M.map_mod local in
+    {{ eval local 🔽
+      tt,
+      forall (z : Z),
+      0 <= z < 64 ->
+      exists (b : bool),
+      (local.(KeccakCols.a_prime_prime_0_0_bits).(Array.get) z) = Z.b2z b
+    }}.
+  Proof.
+    unfold eval.
+    eapply Run.Implies. {
+      repeat (econstructor || intros).
+    }
+    sfirstorder.
+  Qed.
+End a_prime_prime_0_0_bits_bools.
 
 (*
   builder.assert_zeros::<U64_LIMBS, _>(array::from_fn(|limb| {
@@ -528,47 +535,49 @@ Qed.
       computed_a_prime_prime_0_0_limb - local.a_prime_prime[0][0][limb]
   }));
 *)
-Definition eval_assert_a_prime_prime_0_0_limbs {p} `{Prime p}
-    (local : KeccakCols.t) :
-    M.t unit :=
-  M.assert_zeros (N := U64_LIMBS) {|
-    Array.get limb :=
-      let computed_a_prime_prime_0_0_limb : Z :=
-        let l : list nat :=
-          List.rev (
-            List.seq
-              (Z.to_nat (limb * BITS_PER_LIMB))
-              (Z.to_nat (limb * BITS_PER_LIMB + BITS_PER_LIMB))
-            ) in
-        Lists.List.fold_left (fun acc (z : nat) =>
-          let z : Z := Z.of_nat z in
-          BinOp.add (BinOp.mul 2 acc) (local.(KeccakCols.a_prime_prime_0_0_bits).(Array.get) z)
-        ) l 0 in
-      BinOp.sub
-        computed_a_prime_prime_0_0_limb
-        (((local.(KeccakCols.a_prime_prime).(Array.get) 0).(Array.get) 0).(Array.get) limb)
-  |}.
+Module a_prime_prime_0_0_limbs.
+  Definition eval {p} `{Prime p}
+      (local : KeccakCols.t) :
+      M.t unit :=
+    M.assert_zeros (N := U64_LIMBS) {|
+      Array.get limb :=
+        let computed_a_prime_prime_0_0_limb : Z :=
+          let l : list nat :=
+            List.rev (
+              List.seq
+                (Z.to_nat (limb * BITS_PER_LIMB))
+                (Z.to_nat (limb * BITS_PER_LIMB + BITS_PER_LIMB))
+              ) in
+          Lists.List.fold_left (fun acc (z : nat) =>
+            let z : Z := Z.of_nat z in
+            BinOp.add (BinOp.mul 2 acc) (local.(KeccakCols.a_prime_prime_0_0_bits).(Array.get) z)
+          ) l 0 in
+        BinOp.sub
+          computed_a_prime_prime_0_0_limb
+          (((local.(KeccakCols.a_prime_prime).(Array.get) 0).(Array.get) 0).(Array.get) limb)
+    |}.
 
-Lemma eval_assert_a_prime_prime_0_0_limbs_implies {p} `{Prime p}
-    (local : KeccakCols.t) :
-    let local := M.map_mod local in
-  {{ eval_assert_a_prime_prime_0_0_limbs local 🔽
-    tt,
-    let a_prime_prime_0_0' : Array.t Z U64_LIMBS :=
-      Limbs.of_bools U64_LIMBS BITS_PER_LIMB
-        local.(KeccakCols.a_prime_prime_0_0_bits) in
-    forall (limb : Z),
-    0 <= limb < U64_LIMBS ->
-    ((local.(KeccakCols.a_prime_prime).(Array.get) 0).(Array.get) 0).(Array.get) limb =
-    a_prime_prime_0_0'.(Array.get) limb
-  }}.
-Proof.
-  unfold eval_assert_a_prime_prime_0_0_limbs.
-  eapply Run.Implies. {
-    repeat (econstructor || intros).
-  }
-  hauto l: on.
-Qed.
+  Lemma implies {p} `{Prime p}
+      (local : KeccakCols.t) :
+      let local := M.map_mod local in
+    {{ eval local 🔽
+      tt,
+      let a_prime_prime_0_0' : Array.t Z U64_LIMBS :=
+        Limbs.of_bools U64_LIMBS BITS_PER_LIMB
+          local.(KeccakCols.a_prime_prime_0_0_bits) in
+      forall (limb : Z),
+      0 <= limb < U64_LIMBS ->
+      ((local.(KeccakCols.a_prime_prime).(Array.get) 0).(Array.get) 0).(Array.get) limb =
+      a_prime_prime_0_0'.(Array.get) limb
+    }}.
+  Proof.
+    unfold eval.
+    eapply Run.Implies. {
+      repeat (econstructor || intros).
+    }
+    hauto l: on.
+  Qed.
+End a_prime_prime_0_0_limbs.
 
 (*
   let get_xored_bit = |i| {
@@ -605,50 +614,52 @@ Definition get_xored_bit {p} `{Prime p}
       computed_a_prime_prime_prime_0_0_limb - local.a_prime_prime_prime_0_0_limbs[limb]
   }));
 *)
-Definition eval_assert_a_prime_prime_prime_0_0_limbs {p} `{Prime p}
-    (local : KeccakCols.t) :
-    M.t unit :=
-  M.assert_zeros (N := U64_LIMBS) {|
-    Array.get limb :=
-      let computed_a_prime_prime_prime_0_0_limb : Z :=
-        let l : list nat :=
-          List.rev (
-            List.seq
-              (Z.to_nat (limb * BITS_PER_LIMB))
-              (Z.to_nat (limb * BITS_PER_LIMB + BITS_PER_LIMB))
-            ) in
-        Lists.List.fold_left (fun acc (z : nat) =>
-          let z : Z := Z.of_nat z in
-          BinOp.add (BinOp.mul 2 acc) (get_xored_bit local z)
-        ) l 0 in
-      BinOp.sub
-        computed_a_prime_prime_prime_0_0_limb
-        (Array.get local.(KeccakCols.a_prime_prime_prime_0_0_limbs) limb)
-  |}.
+Module a_prime_prime_prime_0_0_limbs.
+  Definition eval {p} `{Prime p}
+      (local : KeccakCols.t) :
+      M.t unit :=
+    M.assert_zeros (N := U64_LIMBS) {|
+      Array.get limb :=
+        let computed_a_prime_prime_prime_0_0_limb : Z :=
+          let l : list nat :=
+            List.rev (
+              List.seq
+                (Z.to_nat (limb * BITS_PER_LIMB))
+                (Z.to_nat (limb * BITS_PER_LIMB + BITS_PER_LIMB))
+              ) in
+          Lists.List.fold_left (fun acc (z : nat) =>
+            let z : Z := Z.of_nat z in
+            BinOp.add (BinOp.mul 2 acc) (get_xored_bit local z)
+          ) l 0 in
+        BinOp.sub
+          computed_a_prime_prime_prime_0_0_limb
+          (Array.get local.(KeccakCols.a_prime_prime_prime_0_0_limbs) limb)
+    |}.
 
-Lemma eval_assert_a_prime_prime_prime_0_0_limbs_implies {p} `{Prime p}
-    (local : KeccakCols.t) :
-    let local := M.map_mod local in
-  {{ eval_assert_a_prime_prime_prime_0_0_limbs local 🔽
-    tt,
-    let a_prime_prime_prime_0_0_limb' : Array.t Z U64_LIMBS :=
-      Limbs.of_bools U64_LIMBS BITS_PER_LIMB
-        {|
-          Array.get z :=
-            get_xored_bit local z;
-        |} in
-    forall (limb : Z),
-    0 <= limb < U64_LIMBS ->
-    Array.get local.(KeccakCols.a_prime_prime_prime_0_0_limbs) limb =
-    a_prime_prime_prime_0_0_limb'.(Array.get) limb
-  }}.
-Proof.
-  unfold eval_assert_a_prime_prime_prime_0_0_limbs.
-  eapply Run.Implies. {
-    repeat (econstructor || intros).
-  }
-  hauto l: on.
-Qed.
+  Lemma implies {p} `{Prime p}
+      (local : KeccakCols.t) :
+      let local := M.map_mod local in
+    {{ eval local 🔽
+      tt,
+      let a_prime_prime_prime_0_0_limb' : Array.t Z U64_LIMBS :=
+        Limbs.of_bools U64_LIMBS BITS_PER_LIMB
+          {|
+            Array.get z :=
+              get_xored_bit local z;
+          |} in
+      forall (limb : Z),
+      0 <= limb < U64_LIMBS ->
+      Array.get local.(KeccakCols.a_prime_prime_prime_0_0_limbs) limb =
+      a_prime_prime_prime_0_0_limb'.(Array.get) limb
+    }}.
+  Proof.
+    unfold eval.
+    eapply Run.Implies. {
+      repeat (econstructor || intros).
+    }
+    hauto l: on.
+  Qed.
+End a_prime_prime_prime_0_0_limbs.
 
 (*
   for x in 0..5 {
@@ -662,57 +673,59 @@ Qed.
       }
   }
 *)
-Definition eval_assert_a_prime_prime_prime_next_a {p} `{Prime p}
-    (local next : KeccakCols.t)
-    (is_transition : bool) :
-    M.t unit :=
-  let final_step := local.(KeccakCols.step_flags).(Array.get) (NUM_ROUNDS - 1) in
-  let not_final_step := BinOp.sub 1 final_step in
-  M.for_in_zero_to_n 5 (fun x =>
-  M.for_in_zero_to_n 5 (fun y =>
-    M.when_bool is_transition (
-    M.when not_final_step (
-      M.assert_zeros (N := U64_LIMBS) {|
-        Array.get limb :=
-          BinOp.sub
-            (Impl_KeccakCols.a_prime_prime_prime local y x limb)
-            (Array.get (Array.get (Array.get next.(KeccakCols.a) y) x) limb)
-      |}
-    ))
-  )).
+Module a_prime_prime_prime_next_a.
+  Definition eval {p} `{Prime p}
+      (local next : KeccakCols.t)
+      (is_transition : bool) :
+      M.t unit :=
+    let final_step := local.(KeccakCols.step_flags).(Array.get) (NUM_ROUNDS - 1) in
+    let not_final_step := BinOp.sub 1 final_step in
+    M.for_in_zero_to_n 5 (fun x =>
+    M.for_in_zero_to_n 5 (fun y =>
+      M.when_bool is_transition (
+      M.when not_final_step (
+        M.assert_zeros (N := U64_LIMBS) {|
+          Array.get limb :=
+            BinOp.sub
+              (Impl_KeccakCols.a_prime_prime_prime local y x limb)
+              (Array.get (Array.get (Array.get next.(KeccakCols.a) y) x) limb)
+        |}
+      ))
+    )).
 
-Lemma eval_assert_a_prime_prime_prime_next_a_implies {p} `{Prime p}
-    (local next : KeccakCols.t) :
-  let local := M.map_mod local in
-  let next := M.map_mod next in
-  let final_step := local.(KeccakCols.step_flags).(Array.get) (NUM_ROUNDS - 1) in
-  let not_final_step := BinOp.sub 1 final_step in
-  not_final_step <> 0 ->
-  {{ eval_assert_a_prime_prime_prime_next_a local next true 🔽
-    tt,
-    forall (y x : Z),
-    0 <= y < 5 ->
-    0 <= x < 5 ->
-    forall (limb : Z),
-    0 <= limb < U64_LIMBS ->
-    Impl_KeccakCols.a_prime_prime_prime local y x limb =
-    Array.get (Array.get (Array.get next.(KeccakCols.a) y) x) limb
-  }}.
-Proof.
-  intros * H_not_final_step.
-  unfold eval_assert_a_prime_prime_prime_next_a.
-  eapply Run.Implies. {
-    eapply Run.ForInZeroToN. {
-      intros.
+  Lemma implies {p} `{Prime p}
+      (local next : KeccakCols.t) :
+    let local := M.map_mod local in
+    let next := M.map_mod next in
+    let final_step := local.(KeccakCols.step_flags).(Array.get) (NUM_ROUNDS - 1) in
+    let not_final_step := BinOp.sub 1 final_step in
+    not_final_step <> 0 ->
+    {{ eval local next true 🔽
+      tt,
+      forall (y x : Z),
+      0 <= y < 5 ->
+      0 <= x < 5 ->
+      forall (limb : Z),
+      0 <= limb < U64_LIMBS ->
+      Impl_KeccakCols.a_prime_prime_prime local y x limb =
+      Array.get (Array.get (Array.get next.(KeccakCols.a) y) x) limb
+    }}.
+  Proof.
+    intros * H_not_final_step.
+    unfold eval.
+    eapply Run.Implies. {
       eapply Run.ForInZeroToN. {
         intros.
-        cbn.
-        unfold M.when.
-        repeat unfold final_step, not_final_step, NUM_ROUNDS in *; cbn in *.
-        destruct (_ =? 0) eqn:H_final_step_eq; [lia |].
-        eapply Run.AssertZerosFromFnSub.
+        eapply Run.ForInZeroToN. {
+          intros.
+          cbn.
+          unfold M.when.
+          repeat unfold final_step, not_final_step, NUM_ROUNDS in *; cbn in *.
+          destruct (_ =? 0) eqn:H_final_step_eq; [lia |].
+          eapply Run.AssertZerosFromFnSub.
+        }
       }
     }
-  }
-  sfirstorder.
-Qed.
+    sfirstorder.
+  Qed.
+End a_prime_prime_prime_next_a.
