Garden/Plonky3/keccak/columns.v
@@ -43,6 +43,38 @@ Module KeccakCols.
       KeccakCols.a_prime_prime_prime_0_0_limbs := M.map_mod x.(KeccakCols.a_prime_prime_prime_0_0_limbs);
     |};
   }.
+
+  Definition get_preimage (local : KeccakCols.t) (x y limb : Z) : Z :=
+    ((local.(KeccakCols.preimage).(Array.get) y).(Array.get) x).(Array.get) limb.
+
+  Definition get_a (local : KeccakCols.t) (x y limb : Z) : Z :=
+    ((local.(KeccakCols.a).(Array.get) y).(Array.get) x).(Array.get) limb.
+
+  Definition get_c (local : KeccakCols.t) (x z : Z) : Z :=
+    ((local.(KeccakCols.c).(Array.get) x).(Array.get) z).
+
+  Definition get_c_prime (local : KeccakCols.t) (x z : Z) : Z :=
+    ((local.(KeccakCols.c_prime).(Array.get) x).(Array.get) z).
+
+  Definition get_a_prime (local : KeccakCols.t) (x y z : Z) : Z :=
+    (((local.(KeccakCols.a_prime).(Array.get) y).(Array.get) x).(Array.get) z).
+
+  Definition get_a_prime_prime (local : KeccakCols.t) (x y limb : Z) : Z :=
+    ((local.(KeccakCols.a_prime_prime).(Array.get) y).(Array.get) x).(Array.get) limb.
+
+  Module Bool.
+    Definition get_a (local : KeccakCols.t) (x y z : Z) : bool :=
+      Limbs.get_bit BITS_PER_LIMB ((local.(KeccakCols.a).(Array.get) y).(Array.get) x) z.
+
+    Definition get_c (local : KeccakCols.t) (x z : Z) : bool :=
+      Z.odd ((get_c local x z)).
+
+    Definition get_c_prime (local : KeccakCols.t) (x z : Z) : bool :=
+      Z.odd ((get_c_prime local x z)).
+
+    Definition get_a_prime (local : KeccakCols.t) (x y z : Z) : bool :=
+      Z.odd ((get_a_prime local x y z)).
+  End Bool.
 End KeccakCols.
 
 Module Impl_KeccakCols.
